fixes and cleanup after rebase part1

ExistentialRules/ChaseSequence/CoreChase/Basic.lean
@@ -1,4 +1,5 @@
-import ExistentialRules.ChaseSequence.Basic
+import ExistentialRules.ChaseSequence.ChaseBranch
+
 import ExistentialRules.Models.Basic
 import ExistentialRules.Models.Cores
 import PossiblyInfiniteTrees.PossiblyInfiniteTree.FiniteDegreeTree.Basic
@@ -12,6 +13,8 @@ import ExistentialRules.ChaseSequence.Universality
 import ExistentialRules.ChaseSequence.Deterministic
 
 import ExistentialRules.ChaseSequence.CoreChase.Util
+
+import BasicLeanDatastructures.List.EraseDupsKeepRight
 
 
 variable {sig : Signature} [DecidableEq sig.P] [DecidableEq sig.C] [DecidableEq sig.V]
@@ -33,63 +36,16 @@ namespace Fact
   @[grind]
   theorem FactGeneralizedAtomEq (f : Fact sig) (ga : GeneralizedAtom sig (GroundTerm sig)) : f = ga ↔ f.predicate = ga.predicate ∧ f.terms = ga.terms := by
       constructor
-      intro eq
-      rw [eq]
-      exact ⟨rfl, rfl⟩
-      intro ⟨eq_p, eq_t⟩
-      rw [GeneralizedAtom.mk.injEq]
-      exact ⟨eq_p, eq_t⟩
+      · intro eq
+        rw [eq]
+        exact ⟨rfl, rfl⟩
+      · intro ⟨eq_p, eq_t⟩
+        rw [GeneralizedAtom.mk.injEq]
+        exact ⟨eq_p, eq_t⟩
 
 end Fact
 
-
-namespace FactSet
-
-  @[grind]
-  theorem applyFactSetIdEq (fs : FactSet sig) : fs = GroundTermMapping.applyFactSet id fs := by
-    unfold GroundTermMapping.applyFactSet TermMapping.apply_generalized_atom_set
-    apply Set.ext
-    intro f
-    constructor
-    intro f_in
-    exists f
-    constructor
-    exact f_in
-    exact Fact.applyFactIdEq f (TermMapping.apply_generalized_atom id f) rfl
-    intro f_in_map
-    rcases f_in_map with ⟨ga, ga_in, ga_eq⟩
-    unfold TermMapping.apply_generalized_atom at ga_eq
-    rw [GeneralizedAtom.mk.injEq] at ga_eq
-    simp only [List.map_id_fun, id_eq] at ga_eq
-    apply Classical.byContradiction
-    intro contra
-    have neq : ga ≠ f := ne_of_mem_of_not_mem ga_in contra
-    have := Fact.FactGeneralizedAtomEq f ga
-    rw [← this] at ga_eq
-    exact neq (id (Eq.symm ga_eq))
-
-end FactSet
-
-namespace ChaseNode
-
-  def ChaseNode.isWeakCore {obs : ObsoletenessCondition sig} (node : ChaseNode obs rules) :
-    Prop := FactSet.isWeakCore node.facts.val
-
-  def ChaseNode.isStrongCore {obs : ObsoletenessCondition sig} (node : ChaseNode obs rules) :
-  Prop := FactSet.isStrongCore node.facts.val
-
-end ChaseNode
-
-
 namespace GroundTermMapping
-
-  @[grind]
-  theorem id_is_id_on_const (h : GroundTermMapping sig) (h_eq : h = id) : h.isIdOnConstants := by
-    rw [h_eq]
-    intro gt
-    split
-    next => trivial
-    next => trivial
 
   def isIsomorphism (h : GroundTermMapping sig) (A B : FactSet sig) : Prop :=
       h.isHomomorphism A B ∧ Function.injective_for_domain_set h A.terms ∧ Function.surjective_for_domain_and_image_set h A.terms B.terms ∧ h.strong A.terms A B
@@ -99,13 +55,13 @@ namespace GroundTermMapping
   theorem homApplyFactFunctionFreeId (fs1 fs2 : FactSet sig) (f : Fact sig) (f_is_ff : f.isFunctionFree) (gtm : GroundTermMapping sig) (gtm_hom : gtm.isHomomorphism fs1 fs2) : gtm.applyFact f = f := by
       rw [GeneralizedAtom.mk.injEq]
       constructor
-      rfl
-      apply List.map_id_of_id_on_all_mem
-      intro gt gt_in
-      specialize f_is_ff gt gt_in
-      rcases f_is_ff with ⟨c, c_eq⟩
-      rw [c_eq]
-      apply gtm_hom.left (.const c)
+      · rfl
+      · apply List.map_id_of_id_on_all_mem
+        intro gt gt_in
+        specialize f_is_ff gt gt_in
+        rcases f_is_ff with ⟨c, c_eq⟩
+        rw [c_eq]
+        exact @gtm_hom.left c
 
   @[simp, grind]
   theorem homApplyFactSetFunctionFreeId (fs1 fs2 : FactSet sig) (fs1_is_ff : fs1.isFunctionFree) (gtm : GroundTermMapping sig) (gtm_hom : gtm.isHomomorphism fs1 fs2) : gtm.applyFactSet fs1 = fs1 := by
@@ -113,15 +69,15 @@ namespace GroundTermMapping
     apply Set.ext
     intro f
     constructor
-    intro ⟨ff, ff_in, ff_eq⟩
-    have := homApplyFactFunctionFreeId fs1 fs2 ff (fs1_is_ff ff ff_in) gtm gtm_hom
-    grind
-    intro h
-    exists f
-    constructor
-    exact h
-    rw [← GroundTermMapping.applyFact.eq_def]
-    rw [homApplyFactFunctionFreeId fs1 fs2 f (fs1_is_ff f h) gtm gtm_hom]
+    · intro ⟨ff, ff_in, ff_eq⟩
+      have := homApplyFactFunctionFreeId fs1 fs2 ff (fs1_is_ff ff ff_in) gtm gtm_hom
+      grind
+    · intro h
+      exists f
+      constructor
+      exact h
+      rw [← GroundTermMapping.applyFact.eq_def]
+      rw [homApplyFactFunctionFreeId fs1 fs2 f (fs1_is_ff f h) gtm gtm_hom]
 
 
   @[grind]
@@ -130,23 +86,23 @@ namespace GroundTermMapping
       unfold GroundTermMapping.applyFact
       rw [GeneralizedAtom.mk.injEq]
       constructor
-      rfl
-      apply List.map_id_of_id_on_all_mem
-      intro gt gt_in
-      unfold GroundTermMapping.isHomomorphism at gtm_hom
-      have db_funfree := kb.db.toFactSet.property.right
-      unfold FactSet.isFunctionFree at db_funfree
-      specialize db_funfree f f_in_db
-      unfold Fact.isFunctionFree at db_funfree
-      specialize db_funfree gt gt_in
-      rcases db_funfree with ⟨c, c_eq⟩
-      rcases f_in_db with ⟨ff, ff_in, ff_eq⟩
-      unfold FunctionFreeFact.toFact at ff_eq
-      rw [GeneralizedAtom.mk.injEq] at ff_eq
-      rcases ff_eq with ⟨ff_pred_eq, ff_map_eq⟩
-      rcases gtm_hom with ⟨gtm_c, gtm_sub⟩
-      rw [c_eq]
-      apply gtm_c (.const c)
+      · rfl
+      · apply List.map_id_of_id_on_all_mem
+        intro gt gt_in
+        unfold GroundTermMapping.isHomomorphism at gtm_hom
+        have db_funfree := kb.db.toFactSet.property.right
+        unfold FactSet.isFunctionFree at db_funfree
+        specialize db_funfree f f_in_db
+        unfold Fact.isFunctionFree at db_funfree
+        specialize db_funfree gt gt_in
+        rcases db_funfree with ⟨c, c_eq⟩
+        rcases f_in_db with ⟨ff, ff_in, ff_eq⟩
+        unfold FunctionFreeFact.toFact at ff_eq
+        rw [GeneralizedAtom.mk.injEq] at ff_eq
+        rcases ff_eq with ⟨ff_pred_eq, ff_map_eq⟩
+        rcases gtm_hom with ⟨gtm_c, gtm_sub⟩
+        rw [c_eq]
+        exact @gtm_c c
 
   @[grind]
   theorem hom_on_db_term_id (t : GroundTerm sig) (gtm : GroundTermMapping sig) (gtm_hom : gtm.isHomomorphism kb.db.toFactSet.val kb.db.toFactSet.val) (t_in_db_terms : t ∈ kb.db.toFactSet.val.terms) :
@@ -158,24 +114,7 @@ namespace GroundTermMapping
       specialize db_funfree f f_in t f_in_ter
       rcases db_funfree with ⟨c, c_eq⟩
       rw [c_eq]
-      apply gtm_hom.left (.const c)
-
-  @[grind]
-  theorem exHomSubToSet (A B : FactSet sig) (sub : A ⊆ B) : ∃ (h : GroundTermMapping sig), h.isHomomorphism A B := by
-    exists id
-    constructor
-    intro gt
-    simp only [id_eq]
-    split
-    next => trivial
-    next => trivial
-    intro f f_in
-    specialize sub f
-    apply sub
-    rcases f_in with ⟨g, g_in_a, g_in_ida⟩
-    have eq := Fact.applyFactIdEq g f (Eq.symm g_in_ida)
-    rw [← eq]
-    exact g_in_a
+      exact @gtm_hom.left c
 
 
   @[grind]
@@ -200,10 +139,273 @@ namespace GroundTermMapping
   theorem subPreservesHom (A B C : FactSet sig) (sub : C ⊆ A) (h : GroundTermMapping sig) (h_hom : h.isHomomorphism  A B) : h.isHomomorphism C B := by
     rcases h_hom with ⟨idc, af⟩
     constructor
-    exact idc
-    intro f f_in_afc
-    have f_in_afb := memApplyFactSetIfMemApplyFactSetSubSet h C A
-    specialize f_in_afb f f_in_afc sub
-    exact af f f_in_afb
+    · exact idc
+    · intro f f_in_afc
+      have f_in_afb := memApplyFactSetIfMemApplyFactSetSubSet h C A
+      specialize f_in_afb f f_in_afc sub
+      exact af f f_in_afb
+
+  theorem id_is_hom {fs : FactSet sig} : GroundTermMapping.isHomomorphism id fs fs := by
+    constructor
+    · exact Subtype.ext rfl
+    · intro f ⟨e, mem, eq⟩
+      rw [TermMapping.apply_generalized_atom_eq_self_of_id_on_terms] at eq
+      . grind
+      . simp
 
 end GroundTermMapping
+
+
+namespace FactSet
+
+  @[simp, grind =]
+  theorem applyFactSetIdEq (fs : FactSet sig) : GroundTermMapping.applyFactSet id fs = fs := by
+    unfold GroundTermMapping.applyFactSet TermMapping.apply_generalized_atom_set
+    apply Set.ext
+    intro f
+    constructor
+    · intro f_in_map
+      rcases f_in_map with ⟨ga, ga_in, ga_eq⟩
+      unfold TermMapping.apply_generalized_atom at ga_eq
+      rw [GeneralizedAtom.mk.injEq] at ga_eq
+      simp only [List.map_id_fun, id_eq] at ga_eq
+      grind
+    · intro f_in
+      exists f
+      exact ⟨f_in, Eq.symm (Fact.applyFactIdEq f (TermMapping.apply_generalized_atom id f) rfl)⟩
+
+  @[grind]
+  theorem exHomSubToSet (A B : FactSet sig) (sub : A ⊆ B) : ∃ (h : GroundTermMapping sig), h.isHomomorphism A B := by
+
+    exists id
+    constructor
+    · intro gt
+      simp only [id_eq]
+    · intro f f_in
+      grind
+
+  theorem empty_set_is_weak_core : (∅ : FactSet sig).isWeakCore := by
+    intro gtm ghom
+    constructor
+    · intro _ _ contra _
+      contradiction
+    · intro h1 h2 h3 h4 h5
+      unfold FactSet.terms at h3
+      rcases h3 with ⟨_, contra, _⟩
+      contradiction
+
+  theorem homSubset_refl (fs : FactSet sig) : fs.homSubset fs := by
+    constructor
+    . apply Set.subset_refl
+    . exists id
+      exact GroundTermMapping.id_is_hom
+
+  theorem apply_fact_set_monotone (f : GroundTermMapping sig) (A B : FactSet sig) (subset : A ⊆ B):
+    f.applyFactSet B ⊆ A → f.applyFactSet B ⊆ B := by
+      intro h
+      intro e e_in_af_B
+      specialize h e e_in_af_B
+      specialize subset e h
+      exact subset
+
+  @[grind =>]
+  theorem weak_core_of_neq_subset (l : List (Fact sig)):
+    ¬ (∃ (sub : List (Fact sig)), sub ⊆ l ∧ sub.toSet ≠ l.toSet ∧ FactSet.homSubset sub.toSet l.toSet) -> (isWeakCore l.toSet) := by
+      intro h
+      simp only [not_exists] at h
+      intro gtm gtm_hom
+      simp only [not_and, ne_eq] at h
+      have l_set_fin : l.toSet.finite := by exact List.finite_toSet l
+      have inj_str := hom_strong_of_finite_of_injective l.toSet l_set_fin gtm gtm_hom
+
+      specialize h (l.map gtm.applyFact)
+
+      have af_sub_l : List.map gtm.applyFact l ⊆ l := by
+        rw [List.subset_def]
+        intro f f_in_l
+        rw [List.mem_map] at f_in_l
+        rcases f_in_l with ⟨f', f'_in_l, f'_eq⟩
+        rcases gtm_hom with ⟨gtm_c, gtm_af⟩
+
+        specialize gtm_af f
+        rw [← List.mem_toSet]
+        apply gtm_af
+        unfold GroundTermMapping.applyFactSet
+        exists f'
+
+      specialize h af_sub_l
+
+      have hom_subset : homSubset (l.map gtm.applyFact).toSet l.toSet := by
+        rcases gtm_hom with ⟨gtm_c, gtm_af⟩
+        unfold homSubset
+        have : gtm.applyFactSet l.toSet = (List.map gtm.applyFact l).toSet := by
+          apply Set.ext
+          intro e
+          rw [List.mem_toSet, List.mem_map]
+          unfold GroundTermMapping.applyFactSet
+          constructor
+          . intro h2
+            rcases h2 with ⟨f, f_in, f_eq⟩
+            exists f
+          . intro h2
+            rcases h2 with ⟨f, f_in, f_eq⟩
+            exists f
+
+        constructor
+        · rw [← this]
+          exact gtm_af
+        · exists gtm
+          constructor
+          . exact gtm_c
+          . rw [this]; apply Set.subset_refl
+
+      cases Decidable.em (l ⊆ l.map gtm.applyFact) with
+      | inl l_sub_mapped =>
+        have eq : (l.map gtm.applyFact).toSet = l.toSet := by
+          simp_all only [not_true_eq_false, imp_false, Classical.not_not]
+
+        rw [propext (and_iff_right_of_imp inj_str)]
+        let terms_list := (l.flatMap GeneralizedAtom.terms).eraseDupsKeepRight
+        have nodup_terms_list : terms_list.Nodup := by
+          apply List.nodup_eraseDupsKeepRight
+        have mem_terms_list : ∀ e, e ∈ terms_list ↔ e ∈ (terms l.toSet) := by
+          simp only [terms_list]
+          intro e
+          rw [List.mem_eraseDupsKeepRight]
+          unfold FactSet.terms
+          simp only [List.mem_flatMap]
+          constructor
+          . intro h
+            rcases h with ⟨f, f_in_l, e_in_ft⟩
+            exists f
+          . intro h
+            rcases h with ⟨f, f_in_l, e_in_ft⟩
+            exists f
+
+
+        rw [Function.injective_set_list_equiv gtm (terms l.toSet) terms_list mem_terms_list]
+        rw [Function.injective_iff_length_image_eq_of_nodup]
+
+        apply List.length_eraseDupsKeepRight_eq_of_same_elements
+        intro gt
+        specialize mem_terms_list gt
+
+        unfold terms_list at mem_terms_list
+        rw [List.mem_eraseDupsKeepRight] at mem_terms_list
+        rw [mem_terms_list, ← eq]
+
+        have eq2 : gt ∈ List.flatMap GeneralizedAtom.terms (List.map gtm.applyFact l) ↔ gt ∈ terms (List.map gtm.applyFact l).toSet := by grind
+
+        rw [← eq2]
+        unfold terms_list
+
+        rw [← List.mem_map_iff_mem_map_eraseDupsKeepRight]
+        rw [List.map_flatMap, List.flatMap_map]
+
+        constructor
+        · intro h2
+          rw [List.mem_flatMap] at h2
+          rcases h2 with ⟨f, f_in, f_eq⟩
+          rw [List.mem_flatMap]
+          exists f
+        · intro h2
+          rw [List.mem_flatMap]
+          rw [List.mem_flatMap] at h2
+          rcases h2 with ⟨f, f_in, f_eq⟩
+          exists f
+
+        exact nodup_terms_list
+
+      | inr l_not_sub_mapped =>
+        have neq : (l.map gtm.applyFact).toSet ≠ l.toSet := by
+          intro contra
+          apply l_not_sub_mapped
+          intro f f_in_l
+          rw [Set.ext_iff] at contra
+          specialize contra f
+          rw [← List.mem_toSet]
+          rw [contra]
+          rw [List.mem_toSet]
+          exact f_in_l
+
+        specialize h neq
+        contradiction
+
+  theorem exists_weak_core_for_finite_set (length : Nat) (l : List (Fact sig)) (length_l : l.length = length):
+    ∃ (wc : FactSet sig), wc.isWeakCore ∧ wc.homSubset l.toSet := by
+      induction length using Nat.strongRecOn generalizing l with
+        | ind n ih =>
+          by_cases h : (∃ (sub : List (Fact sig)), sub ⊆ l ∧ sub.toSet ≠ l.toSet ∧ FactSet.homSubset sub.toSet l.toSet)
+          . rcases h with ⟨sub', h2, h3, h4⟩
+            let sub := sub'.eraseDupsKeepRight
+            have sub_eq_sub' : sub.toSet = sub'.toSet := by
+              apply funext
+              intro e
+              apply propext
+              change e ∈ sub.toSet ↔ e ∈ sub'.toSet
+              have := @List.mem_toSet _ sub' e
+              rw [this]
+              have := @List.mem_toSet _ sub e
+              rw [this]
+              apply List.mem_eraseDupsKeepRight
+            specialize ih sub.length  -- m < n
+            by_cases n_zero : (n = 0)
+            . exists ∅
+              constructor
+              . apply empty_set_is_weak_core
+              . rw [n_zero] at length_l
+                have : l.toSet = ∅ := by
+                  rw [List.length_eq_zero_iff.mp length_l]
+                  apply Set.ext; intro e; rw [List.mem_toSet, List.mem_nil_iff]; simp [Membership.mem, EmptyCollection.emptyCollection]
+                rw [this]
+                apply homSubset_refl
+            . have x : _ := ih (by
+                rw [← length_l]
+                apply List.length_lt_of_proper_subset
+                . apply List.nodup_eraseDupsKeepRight
+                . intro e e_mem; apply h2; rw [List.mem_eraseDupsKeepRight] at e_mem; exact e_mem
+                . intro contra
+                  apply h3
+                  rw [← contra]
+                  rw [sub_eq_sub']
+              ) sub rfl
+              rcases x with ⟨fs, fs_wc, fs_hom_ss_tl⟩
+              exists fs
+              constructor
+              . exact fs_wc
+              . rw [sub_eq_sub'] at fs_hom_ss_tl
+                rcases fs_hom_ss_tl with ⟨fs_ss_tl, ⟨gtm ,ghom⟩⟩
+                rw [homSubset]
+                constructor
+                have h2' : sub'.toSet ⊆ l.toSet := Set.subset_trans h2 fun e a => a
+                . apply Set.subset_trans fs_ss_tl h2'
+                . rcases h4 with ⟨h4_sub, h4_hom, h4_hom_hom⟩
+                  exists gtm ∘ h4_hom
+                  apply GroundTermMapping.isHomomorphism_compose
+                  . exact h4_hom_hom
+                  . exact ghom
+          -- l.toSet is wc
+          · have x : FactSet.isWeakCore l.toSet := by
+              apply weak_core_of_neq_subset
+              exact h
+            exists l.toSet
+            constructor
+            exact x
+            rw [homSubset]
+            constructor
+            apply Set.subset_refl
+            exists id
+            exact GroundTermMapping.id_is_hom
+
+
+end FactSet
+
+namespace ChaseNode
+
+  def ChaseNode.isWeakCore {obs : ObsolescenceCondition sig} (node : ChaseNode obs rules) :
+    Prop := FactSet.isWeakCore node.facts
+
+  def ChaseNode.isStrongCore {obs : ObsolescenceCondition sig} (node : ChaseNode obs rules) :
+  Prop := FactSet.isStrongCore node.facts
+
+end ChaseNode
