ExistentialRules/ChaseSequence/CoreChase/CoreChaseNode.lean
@@ -1,4 +1,4 @@
-import ExistentialRules.ChaseSequence.Basic
+import ExistentialRules.ChaseSequence.ChaseBranch
 import ExistentialRules.Models.Basic
 import ExistentialRules.Models.Cores
 import PossiblyInfiniteTrees.PossiblyInfiniteTree.FiniteDegreeTree.Basic
@@ -14,7 +14,7 @@ import ExistentialRules.ChaseSequence.CoreChase.Util
 
 variable {sig : Signature} [DecidableEq sig.P] [DecidableEq sig.C] [DecidableEq sig.V]
 variable {kb : KnowledgeBase sig}
-abbrev obs := RestrictedObsoleteness sig
+abbrev obs := RestrictedObsolescence sig
 
 
 structure CoreChaseNode (rules : RuleSet sig) where
@@ -23,12 +23,12 @@ structure CoreChaseNode (rules : RuleSet sig) where
   core : FactSet sig
   is_core : core.isWeakCore
   core_sse : core.homSubset fs
-  origin : Option ((trg : RTrigger obs.toLaxObsoletenessCondition rules) × Fin trg.val.mapped_head.length)
-  fs_contains_origin_result : origin.is_none_or (fun origin => origin.fst.val.mapped_head[origin.snd.val].toSet ⊆ fs)
+  origin : Option ((trg : RTrigger obs.toLaxObsolescenceCondition rules) × Fin trg.val.mapped_head.length)
+  fs_contains_origin_result : ∀ o ∈ origin, o.fst.val.mapped_head[o.snd.val].toSet ⊆ fs
 
 namespace CoreChaseNode
 
-  def origin_result {rules : RuleSet sig}  (node : CoreChaseNode rules) (isSome : node.origin.isSome) : List (Fact sig) :=
+  def origin_result {rules : RuleSet sig} (node : CoreChaseNode rules) (isSome : node.origin.isSome) : List (Fact sig) :=
     let origin := node.origin.get isSome
     origin.fst.val.mapped_head[origin.snd.val]
 
